Add initial axiomatic sequential model

ArchSem/CandidateExecution.lean
@@ -15,7 +15,59 @@ open ArchSem.TerminatingModel
 
 namespace ArchSem.CandidateExecutions
 
-abbrev Rel (α : Type) (cmp : α × α → α × α → Ordering := by exact compare) := Std.ExtTreeSet (α × α) cmp
+section TreeSetHelpers
+
+-- TODO: why is this not in lean standard libs?
+def subset {α : Type} {cmp : α → α → Ordering} [Std.TransCmp cmp]
+    (r₁ r₂ : Std.ExtTreeSet α cmp) : Prop :=
+  ∀ (a : α), a ∈ r₁ → a ∈ r₂
+
+instance {α : Type} {cmp : α → α → Ordering} [Std.TransCmp cmp] [Std.LawfulEqCmp cmp]
+    (r₁ r₂ : Std.ExtTreeSet α cmp)
+    : Decidable (subset r₁ r₂) := by
+  if h : r₁.toList.all (fun a => decide (a ∈ r₂)) = true then
+    apply Decidable.isTrue
+    intro a h_mem
+    have h_all := List.all_eq_true.mp h a (Std.ExtTreeSet.mem_toList.mpr h_mem)
+    simpa using h_all
+  else
+    apply Decidable.isFalse
+    intro h_subset
+    apply h
+    apply List.all_eq_true.mpr
+    intro a h_mem
+    have h_mem' := Std.ExtTreeSet.mem_toList.mp h_mem
+    exact decide_eq_true (h_subset a h_mem')
+
+instance {α : Type} {cmp : α → α → Ordering} [Std.TransCmp cmp]
+    : HasSubset (Std.ExtTreeSet α cmp) where
+  Subset := subset
+
+instance {α : Type} {cmp : α → α → Ordering} [Std.TransCmp cmp] [Std.LawfulEqCmp cmp]
+    (r₁ r₂ : Std.ExtTreeSet α cmp)
+    : Decidable (HasSubset.Subset r₁ r₂) := by
+  change Decidable (subset r₁ r₂)
+  infer_instance
+
+instance {α : Type} {cmp : α → α → Ordering} [Std.TransCmp cmp] [Std.LawfulEqCmp cmp]
+    (s : Std.ExtTreeSet α cmp) (p : α → Prop)
+    [DecidablePred p] : Decidable (∀ x ∈ s, p x) := by
+  if h : s.toList.all (fun x => decide (p x)) = true then
+    apply Decidable.isTrue
+    intro x h_mem
+    exact of_decide_eq_true (List.all_eq_true.mp h x (Std.ExtTreeSet.mem_toList.mpr h_mem))
+  else
+    apply Decidable.isFalse
+    intro h_forall
+    apply h
+    apply List.all_eq_true.mpr
+    intro x h_mem
+    exact decide_eq_true (h_forall x (Std.ExtTreeSet.mem_toList.mp h_mem))
+
+end TreeSetHelpers
+
+abbrev Rel (α : Type) (cmp : α × α → α × α → Ordering := by exact compare)
+  := Std.ExtTreeSet (α × α) cmp
 
 namespace Rel
 
@@ -23,12 +75,164 @@ def union {α : Type} {cmp : α × α → α × α → Ordering} [Std.TransCmp c
     (r₁ r₂ : Rel α cmp) : Rel α cmp :=
   Std.ExtTreeSet.union r₁ r₂
 
-def intersection {α : Type} {cmp : α × α → α × α → Ordering} [Std.TransCmp cmp]
+def inter {α : Type} {cmp : α × α → α × α → Ordering} [Std.TransCmp cmp]
     (r₁ r₂ : Rel α cmp) : Rel α cmp :=
   Std.ExtTreeSet.inter r₁ r₂
 
-end Rel
+def diff {α : Type} {cmp : α × α → α × α → Ordering} [Std.TransCmp cmp]
+    (r₁ r₂ : Rel α cmp) : Rel α cmp :=
+  Std.ExtTreeSet.diff r₁ r₂
 
+def diag {α : Type} {cmp' : α → α → Ordering} [Std.TransCmp cmp']
+    {cmp : α × α → α × α → Ordering} [Std.TransCmp cmp]
+    (s : Std.ExtTreeSet α cmp') : Rel α cmp :=
+  s.foldl (fun acc x => acc.insert (x, x)) Std.ExtTreeSet.empty
+
+def transitiveClosure {α : Type} {cmp : α × α → α × α → Ordering} [Std.TransCmp cmp]
+    (r : Rel α cmp) : Rel α cmp :=
+  let lA := r.toList.foldr (fun (x, y) acc => x :: y :: acc) []
+  lA.foldr
+    (fun k s =>
+      lA.foldl
+        (fun s i =>
+          lA.foldl
+            (fun s j =>
+              if s.contains (i, k) && s.contains (k, j) then s.insert (i, j) else s
+            ) s
+        ) s
+    ) r
+
+-- TODO: use maps to make this faster.
+def seq {α : Type} {cmp : α × α → α × α → Ordering} [Std.TransCmp cmp]
+    [DecidableEq α] (r₁ r₂ : Rel α cmp) : Rel α cmp :=
+  r₁.foldl (fun acc (x, y) =>
+    r₂.foldl (fun acc (y', z) =>
+      if y = y' then acc.insert (x, z) else acc
+    ) acc
+  ) Std.ExtTreeSet.empty
+
+def inv {α : Type} {cmp : α × α → α × α → Ordering} [Std.TransCmp cmp]
+    (r : Rel α cmp) : Rel α cmp :=
+  r.foldl (fun acc (x, y) => acc.insert (y, x)) Std.ExtTreeSet.empty
+
+instance {α : Type} {cmp : α × α → α × α → Ordering} [Std.TransCmp cmp]
+    : Inv (Rel α cmp) where
+  inv := inv
+
+infixl:66 " ; " => seq
+prefix:75 "Δ" => diag
+postfix:76 "⁺" => transitiveClosure
+
+def injective {α : Type} {cmp : α × α → α × α → Ordering} [Std.TransCmp cmp]
+    (r : Rel α cmp) : Prop :=
+  ∀ (x y z : α), (x, z) ∈ r → (y, z) ∈ r → x = y
+
+instance {α : Type} {cmp : α × α → α × α → Ordering}
+    [DecidableEq α] [Std.LawfulEqCmp cmp] [Std.TransCmp cmp]
+    (r : Rel α cmp) : Decidable (injective r) := by
+  if h : r.toList.all (fun arrow₁ =>
+      r.toList.all (fun arrow₂ => decide (arrow₁.snd = arrow₂.snd → arrow₁.fst = arrow₂.fst))) = true then
+    apply Decidable.isTrue
+    intro x y z h_xz h_yz
+    have h_outer := List.all_eq_true.mp h (x, z) (Std.ExtTreeSet.mem_toList.mpr h_xz)
+    have h_inner := List.all_eq_true.mp h_outer (y, z) (Std.ExtTreeSet.mem_toList.mpr h_yz)
+    exact (of_decide_eq_true h_inner) rfl
+  else
+    apply Decidable.isFalse
+    intro h_injective
+    apply h
+    apply List.all_eq_true.mpr
+    intro arrow₁ h_arrow₁
+    apply List.all_eq_true.mpr
+    intro arrow₂ h_arrow₂
+    cases arrow₁ with
+    | mk x z =>
+      cases arrow₂ with
+      | mk y z' =>
+        apply decide_eq_true
+        intro h_z
+        subst h_z
+        exact h_injective x y z (Std.ExtTreeSet.mem_toList.mp h_arrow₁) (Std.ExtTreeSet.mem_toList.mp h_arrow₂)
+
+def transitive {α : Type} {cmp : α × α → α × α → Ordering} [Std.TransCmp cmp]
+    (r : Rel α cmp) : Prop :=
+  ∀ (x y z : α), (x, y) ∈ r → (y, z) ∈ r → (x, z) ∈ r
+
+instance {α : Type} {cmp : α × α → α × α → Ordering}
+    [DecidableEq α] [Std.LawfulEqCmp cmp] [Std.TransCmp cmp] (r : Rel α cmp)
+    : Decidable (transitive r) := by
+  if h : r.toList.all (fun arrow₁ =>
+      r.toList.all (fun arrow₂ => decide (arrow₁.snd = arrow₂.fst → (arrow₁.fst, arrow₂.snd) ∈ r))) = true then
+    apply Decidable.isTrue
+    intro x y z h_xy h_yz
+    have h_outer := List.all_eq_true.mp h (x, y) (Std.ExtTreeSet.mem_toList.mpr h_xy)
+    have h_inner := List.all_eq_true.mp h_outer (y, z) (Std.ExtTreeSet.mem_toList.mpr h_yz)
+    exact (of_decide_eq_true h_inner) rfl
+  else
+    apply Decidable.isFalse
+    intro h_transitive
+    apply h
+    apply List.all_eq_true.mpr
+    intro arrow₁ h_arrow₁
+    apply List.all_eq_true.mpr
+    intro arrow₂ h_arrow₂
+    cases arrow₁ with
+    | mk x y =>
+      cases arrow₂ with
+      | mk y' z =>
+        apply decide_eq_true
+        intro h_y
+        change y = y' at h_y
+        subst h_y
+        exact h_transitive x y z (Std.ExtTreeSet.mem_toList.mp h_arrow₁) (Std.ExtTreeSet.mem_toList.mp h_arrow₂)
+
+def irreflexive {α : Type} {cmp : α × α → α × α → Ordering} [Std.TransCmp cmp]
+    (r : Rel α cmp) : Prop :=
+  ∀ (x : α), (x, x) ∉ r
+
+instance {α : Type} {cmp : α × α → α × α → Ordering}
+    [DecidableEq α] [Std.LawfulEqCmp cmp] [Std.TransCmp cmp]
+    (r : Rel α cmp) : Decidable (irreflexive r) := by
+  if h : r.toList.all (fun arrow => decide (arrow.fst ≠ arrow.snd)) = true then
+    apply Decidable.isTrue
+    intro x h_xx
+    have h_ne := List.all_eq_true.mp h (x, x) (Std.ExtTreeSet.mem_toList.mpr h_xx)
+    exact (of_decide_eq_true h_ne) rfl
+  else
+    apply Decidable.isFalse
+    intro h_irreflexive
+    apply h
+    apply List.all_eq_true.mpr
+    intro arrow h_arrow
+    cases arrow with
+    | mk x y =>
+      apply decide_eq_true
+      intro h_xy
+      change x = y at h_xy
+      subst h_xy
+      exact h_irreflexive x (Std.ExtTreeSet.mem_toList.mp h_arrow)
+
+def acyclic {α : Type} {cmp : α × α → α × α → Ordering} [Std.TransCmp cmp]
+    (r : Rel α cmp) : Prop :=
+  r⁺.irreflexive
+
+instance {α : Type} {cmp : α × α → α × α → Ordering}
+    [DecidableEq α] [Std.LawfulEqCmp cmp] [Std.TransCmp cmp]
+    (r : Rel α cmp) : Decidable (acyclic r) := by
+  rw [acyclic]
+  infer_instance
+
+def domain {cmp : α × α → α × α → Ordering} [Std.TransCmp cmp]
+  {cmp' : α → α → Ordering} [Std.TransCmp cmp']
+  (r : Rel α cmp) : Std.ExtTreeSet α cmp' :=
+  r.foldr (fun (x,_) s => s.insert x) Std.ExtTreeSet.empty
+
+def range {cmp : α × α → α × α → Ordering} [Std.TransCmp cmp]
+  {cmp' : α → α → Ordering} [Std.TransCmp cmp']
+  (r : Rel α cmp) : Std.ExtTreeSet α cmp' :=
+  r.foldr (fun (_,y) s => s.insert y) Std.ExtTreeSet.empty
+
+end Rel
 
 abbrev IMon [Arch] := FreeM (InstructionEffect ⊕ FinChoice)
 def IEvent [Arch] : Type := FreeM.Event InstructionEffect
@@ -66,6 +270,10 @@ def getMemRequest (ev : IEvent) : Option MemRequest :=
 def getAddr (ev : IEvent) : Option Address := do
   let memReq ← ev.getMemRequest
   return memReq.address
+
+def getSize (ev : IEvent) : Option Nat := do
+  let memReq ← ev.getMemRequest
+  return memReq.size
 
 def getMemValue (ev : IEvent) : Option (Σ n : Nat, BitVec (8 * n)) :=
   match h : ev.call with
@@ -105,7 +313,7 @@ def getTransEnd (ev : IEvent) : Option Arch.trans_end :=
 
 section IsReg
 
-variable (ev : IEvent) (p : (r : Arch.register) → Option Arch.sys_reg_id → Arch.register_type r → Prop)
+variable (p : (r : Arch.register) → Option Arch.sys_reg_id → Arch.register_type r → Prop) (ev : IEvent)
 
 def is_reg_read_with : Prop
   := match h : ev.call with
@@ -116,7 +324,7 @@ def is_reg_read_with : Prop
     p reg racc val
   | _ => False
 
-instance [h : ∀ r acc v, Decidable (p r acc v)] : Decidable (is_reg_read_with ev p) := by
+instance [h : ∀ r acc v, Decidable (p r acc v)] : Decidable (is_reg_read_with p ev) := by
   rw [is_reg_read_with] ; split
   · apply h
   · exact Decidable.isFalse False.elim
@@ -126,17 +334,18 @@ def is_reg_write_with : Prop
   | .regWrite reg racc val => p reg racc val
   | _ => False
 
-instance [h : ∀ r acc v, Decidable (p r acc v)] : Decidable (is_reg_write_with ev p) := by
+instance [h : ∀ r acc v, Decidable (p r acc v)] : Decidable (is_reg_write_with p ev) := by
   rw [is_reg_write_with] ; split
   · apply h
   · exact Decidable.isFalse False.elim
 
-def is_reg_event_with : Prop := is_reg_read_with ev p ∨ is_reg_write_with ev p
+def is_reg_event_with : Prop := is_reg_read_with p ev ∨ is_reg_write_with p ev
 
 end IsReg
 
-def is_mem_read_req_with (ev : IEvent)
+def is_mem_read_req_with
     (p : (req : MemRequest) → Except Arch.abort (BitVec (8 * req.size) × BitVec (req.numTag)) → Prop)
+    (ev : IEvent)
   := match h : ev.call with
   | .memRead req =>
     let h_eq : Except Arch.abort (BitVec (8 * req.size) × BitVec req.numTag) = Effect.ret ev.call := by
@@ -144,37 +353,39 @@ def is_mem_read_req_with (ev : IEvent)
     p req (h_eq ▸ ev.ret)
   | _ => False
 
-instance [h : ∀ req res, Decidable (p req res)] : Decidable (is_mem_read_req_with ev p) := by
+instance [h : ∀ req res, Decidable (p req res)] : Decidable (is_mem_read_req_with p ev) := by
   rw [is_mem_read_req_with] ; split
   · apply h
   · exact Decidable.isFalse False.elim
 
-def is_mem_read_with (ev : IEvent)
-    (p : (req : MemRequest) → BitVec (8 * req.size) → BitVec req.numTag → Prop) : Prop
-  := is_mem_read_req_with ev (fun req res => match res with
+def is_mem_read_with
+    (p : (req : MemRequest) → BitVec (8 * req.size) → BitVec req.numTag → Prop)
+    : IEvent → Prop
+  := is_mem_read_req_with (fun req res => match res with
        | .ok val => p req val.fst val.snd
        | .error _ => False)
 
 instance [h : ∀ req val tags, Decidable (p req val tags)]
-    : Decidable (is_mem_read_with ev p) := by
+    : Decidable (is_mem_read_with p ev) := by
   rw [is_mem_read_with, is_mem_read_req_with] ; split
   · split
     · apply h
     · exact Decidable.isFalse False.elim
   · exact Decidable.isFalse False.elim
 
-def is_mem_write_announce_with (ev : IEvent) (p : MemRequest → Prop) :=
+def is_mem_write_announce_with (p : MemRequest → Prop) (ev : IEvent) :=
   match ev.call with
   | .memWriteAnnounce req => p req
   | _ => False
 
-instance [h : ∀ req, Decidable (p req)] : Decidable (is_mem_write_announce_with ev p) := by
+instance [h : ∀ req, Decidable (p req)] : Decidable (is_mem_write_announce_with p ev) := by
   rw [is_mem_write_announce_with] ; split
   · apply h
   · exact Decidable.isFalse False.elim
 
-def is_mem_write_req_with (ev : IEvent)
-    (p : (req : MemRequest) → BitVec (8 * req.size) → BitVec req.numTag → Except Arch.abort Unit → Prop) : Prop
+def is_mem_write_req_with
+    (p : (req : MemRequest) → BitVec (8 * req.size) → BitVec req.numTag → Except Arch.abort Unit → Prop)
+    (ev : IEvent) : Prop
   := match h : ev.call with
   | .memWrite req val tags =>
     let h_eq : Except Arch.abort Unit = Effect.ret ev.call := by
@@ -183,73 +394,96 @@ def is_mem_write_req_with (ev : IEvent)
   | _ => False
 
 instance [h : ∀ req val tags res, Decidable (p req val tags res)]
-    : Decidable (is_mem_write_req_with ev p) := by
+    : Decidable (is_mem_write_req_with p ev) := by
   rw [is_mem_write_req_with] ; split
   · apply h
   · exact Decidable.isFalse False.elim
 
-def is_mem_write_with (ev : IEvent)
-    (p : (req : MemRequest) → BitVec (8 * req.size) → BitVec req.numTag → Prop) : Prop
-  := is_mem_write_req_with ev (fun req val tags res => match res with
+def is_mem_write_with
+    (p : (req : MemRequest) → BitVec (8 * req.size) → BitVec req.numTag → Prop)
+    : IEvent → Prop
+  := is_mem_write_req_with (fun req val tags res => match res with
        | .ok () => p req val tags
        | .error _ => False)
 
 instance [h : ∀ req val tags, Decidable (p req val tags)]
-    : Decidable (is_mem_write_with ev p) := by
+    : Decidable (is_mem_write_with p ev) := by
   rw [is_mem_write_with, is_mem_write_req_with] ; split
   · split
     · apply h
     · exact Decidable.isFalse False.elim
   · exact Decidable.isFalse False.elim
 
-def is_barrier_with (ev : IEvent) (p : Arch.barrier → Prop) : Prop
+def is_barrier_with (p : Arch.barrier → Prop) (ev : IEvent) : Prop
   := match ev.call with
   | .barrier barrier => p barrier
   | _ => False
 
 instance [h : ∀ barrier, Decidable (p barrier)]
-    : Decidable (is_barrier_with ev p) := by
+    : Decidable (is_barrier_with p ev) := by
   rw [is_barrier_with] ; split
   · apply h
   · exact Decidable.isFalse False.elim
 
-def is_cache_op_with (ev : IEvent) (p : Arch.cache_op → Prop) : Prop
+def is_cache_op_with (p : Arch.cache_op → Prop) (ev : IEvent) : Prop
   := match ev.call with
   | .cacheOp op => p op
   | _ => False
 
 instance [h : ∀ op, Decidable (p op)]
-    : Decidable (is_cache_op_with ev p) := by
+    : Decidable (is_cache_op_with p ev) := by
   rw [is_cache_op_with] ; split
   · apply h
   · exact Decidable.isFalse False.elim
 
-def is_tlb_op_with (ev : IEvent) (p : Arch.tlbi → Prop) : Prop
+def is_tlb_op_with (p : Arch.tlbi → Prop) (ev : IEvent) : Prop
   := match ev.call with
   | .tlbOp op => p op
   | _ => False
 
 instance [h : ∀ op, Decidable (p op)]
-    : Decidable (is_tlb_op_with ev p) := by
+    : Decidable (is_tlb_op_with p ev) := by
   rw [is_tlb_op_with] ; split
   · apply h
   · exact Decidable.isFalse False.elim
 
-abbrev is_reg_read (ev : IEvent) := is_reg_read_with ev (fun _ _ _ => True)
-abbrev is_reg_write (ev : IEvent) := is_reg_write_with ev (fun _ _ _ => True)
-abbrev is_reg_event (ev : IEvent) := is_reg_event_with ev (fun _ _ _ => True)
-abbrev is_mem_read_req (ev : IEvent) := is_mem_read_req_with ev (fun _ _ => True)
-abbrev is_mem_read (ev : IEvent) := is_mem_read_with ev (fun _ _ _ => True)
-abbrev is_mem_write_announce (ev : IEvent) := is_mem_write_announce_with ev (fun _ => True)
-abbrev is_mem_write_req (ev : IEvent) := is_mem_write_req_with ev (fun _ _ _ _ => True)
-abbrev is_mem_write (ev : IEvent) := is_mem_write_with ev (fun _ _ _ => True)
-abbrev is_barrier (ev : IEvent) := is_barrier_with ev (fun _ => True)
-abbrev is_cache_op (ev : IEvent) := is_cache_op_with ev (fun _ => True)
-abbrev is_tlb_op (ev : IEvent) := is_tlb_op_with ev (fun _ => True)
+def is_arch_exception (ev : IEvent) : Prop
+  := match ev.call with
+  | .archException _ => True
+  | _ => False
+
+instance : Decidable (is_arch_exception ev) := by
+  rw [is_arch_exception]
+  split <;> infer_instance
+
+def is_return_exception (ev : IEvent) : Prop
+  := match ev.call with
+  | .returnExecption => True
+  | _ => False
+
+instance : Decidable (is_return_exception ev) := by
+  rw [is_return_exception]
+  split <;> infer_instance
+
+abbrev is_reg_read (ev : IEvent) := is_reg_read_with (fun _ _ _ => True) ev
+abbrev is_reg_write (ev : IEvent) := is_reg_write_with (fun _ _ _ => True) ev
+abbrev is_reg_event (ev : IEvent) := is_reg_event_with (fun _ _ _ => True) ev
+abbrev is_mem_read_req (ev : IEvent) := is_mem_read_req_with (fun _ _ => True) ev
+abbrev is_mem_read (ev : IEvent) := is_mem_read_with (fun _ _ _ => True) ev
+abbrev is_mem_write_announce (ev : IEvent) := is_mem_write_announce_with (fun _ => True) ev
+abbrev is_mem_write_req (ev : IEvent) := is_mem_write_req_with (fun _ _ _ _ => True) ev
+abbrev is_mem_write (ev : IEvent) := is_mem_write_with (fun _ _ _ => True) ev
+abbrev is_barrier (ev : IEvent) := is_barrier_with (fun _ => True) ev
+abbrev is_cache_op (ev : IEvent) := is_cache_op_with (fun _ => True) ev
+abbrev is_tlb_op (ev : IEvent) := is_tlb_op_with (fun _ => True) ev
 
 def is_unsupported_event (ev : IEvent) : Prop :=
-  is_mem_read_req_with ev (fun req _ => req.numTag ≠ 0) ∨
-  is_mem_write_req_with ev (fun req _ _ _ => req.numTag ≠ 0)
+  is_mem_read_req_with (fun req _ => req.numTag ≠ 0) ev ∨
+  is_mem_write_req_with (fun req _ _ _ => req.numTag ≠ 0) ev
+
+instance : Decidable (is_unsupported_event ev) := by
+  unfold is_unsupported_event
+  infer_instance
 
 end IEvent
 
@@ -269,34 +503,51 @@ structure Eid where
   tid : Nat
   iid : Nat
   ieid : Nat
-deriving BEq
-
--- TODO: other Eid ordering relations?
+deriving DecidableEq
 
 def Eid.compare (a b : Eid) : Ordering :=
-  if a.tid < b.tid
-  then .lt
-  else if a.tid > b.tid
-  then .gt
-  else if a.iid < b.iid
-  then .lt
-  else if a.iid > b.iid
-  then .gt
-  else if a.ieid < b.ieid
-  then .lt
-  else if a.ieid > b.ieid
-  then .gt
-  else .eq
+  (Ord.compare : (Nat × Nat × Nat) → (Nat × Nat × Nat) → Ordering)
+    (a.tid, a.iid, a.ieid) (b.tid, b.iid, b.ieid)
 
 instance : Ord Eid where
   compare := Eid.compare
 
 instance : Std.TransCmp Eid.compare where
-  isLE_trans := by sorry
-  eq_swap := by sorry
+  isLE_trans := by
+    intro a b c hab hbc
+    simpa only [Eid.compare] using
+      (Std.TransCmp.isLE_trans
+        (cmp := (Ord.compare : (Nat × Nat × Nat) → (Nat × Nat × Nat) → Ordering)) hab hbc)
+  eq_swap := by
+    intro a b
+    simpa only [Eid.compare] using
+      (Std.OrientedCmp.eq_swap
+        (cmp := (Ord.compare : (Nat × Nat × Nat) → (Nat × Nat × Nat) → Ordering))
+        (a := (a.tid, a.iid, a.ieid)) (b := (b.tid, b.iid, b.ieid)))
+
+instance : Std.LawfulEqCmp Eid.compare where
+  compare_self := by
+    intro a
+    simpa only [Eid.compare] using
+      (Std.ReflCmp.compare_self
+        (cmp := (Ord.compare : (Nat × Nat × Nat) → (Nat × Nat × Nat) → Ordering))
+        (a := (a.tid, a.iid, a.ieid)))
+  eq_of_compare := by
+    intro a b h
+    have h_key : (a.tid, a.iid, a.ieid) = (b.tid, b.iid, b.ieid) := by
+      apply Std.LawfulEqCmp.eq_of_compare
+        (cmp := (Ord.compare : (Nat × Nat × Nat) → (Nat × Nat × Nat) → Ordering))
+      simpa only [Eid.compare] using h
+    cases a
+    cases b
+    simp_all
 
 instance : Std.TransCmp (compare : Eid → Eid → Ordering) := by
   change Std.TransCmp Eid.compare
+  infer_instance
+
+instance : Std.LawfulEqCmp (compare : Eid → Eid → Ordering) := by
+  change Std.LawfulEqCmp Eid.compare
   infer_instance
 
 -- TODO: Eid ordering relations
@@ -361,7 +612,7 @@ instance : GetElem (PreCand nThreads) Eid IEvent eid_valid where
        rw [←Option.not_isSome_iff_eq_none] at h_lookup
        contradiction
 
-def collectEid (f : Eid → IEvent → Prop) (p : PreCand nThreads)
+def collectEidWith (f : Eid → IEvent → Prop) (p : PreCand nThreads)
     [h : ∀ eid ev, Decidable (f eid ev)]
     : Std.ExtTreeSet Eid :=
   Std.ExtTreeSet.ofList (
@@ -370,48 +621,52 @@ def collectEid (f : Eid → IEvent → Prop) (p : PreCand nThreads)
     |>.map Prod.fst
   )
 
-def eids (p : PreCand nThreads) : Std.ExtTreeSet Eid := p.collectEid (fun _ _ => True)
+def eids (p : PreCand nThreads) : Std.ExtTreeSet Eid :=
+  p.collectEidWith (fun _ _ => True)
 
 def regReads (p : PreCand nThreads) : Std.ExtTreeSet Eid :=
-  p.collectEid (fun _ ev => IEvent.is_reg_read ev)
+  p.collectEidWith (fun _ ev => IEvent.is_reg_read ev)
 def pcReads (p : PreCand nThreads) : Std.ExtTreeSet Eid :=
-  p.collectEid (fun _ ev => IEvent.is_reg_read_with ev (fun reg _ _ => reg = ArchExtra.register_pc))
+  p.collectEidWith (fun _ ev => IEvent.is_reg_read_with (fun reg _ _ => reg = ArchExtra.register_pc) ev)
 
 def regWrites (p : PreCand nThreads) : Std.ExtTreeSet Eid :=
-  p.collectEid (fun _ ev => IEvent.is_reg_write ev)
+  p.collectEidWith (fun _ ev => IEvent.is_reg_write ev)
 def pcWrites (p : PreCand nThreads) : Std.ExtTreeSet Eid :=
-  p.collectEid (fun _ ev => IEvent.is_reg_write_with ev (fun reg _ _ => reg = ArchExtra.register_pc))
+  p.collectEidWith (fun _ ev => IEvent.is_reg_write_with (fun reg _ _ => reg = ArchExtra.register_pc) ev)
 
 def memReads (p : PreCand nThreads) : Std.ExtTreeSet Eid :=
-  p.collectEid (fun _ ev => IEvent.is_mem_read ev)
+  p.collectEidWith (fun _ ev => IEvent.is_mem_read ev)
 def memReadReqs (p : PreCand nThreads) : Std.ExtTreeSet Eid :=
-  p.collectEid (fun _ ev => IEvent.is_mem_read_req ev)
+  p.collectEidWith (fun _ ev => IEvent.is_mem_read_req ev)
 
 def memReadAborts (p : PreCand nThreads) : Std.ExtTreeSet Eid :=
-  p.collectEid (fun _ ev => IEvent.is_mem_read_req_with ev (fun _ res => not res.isOk))
+  p.collectEidWith (fun _ ev => IEvent.is_mem_read_req_with (fun _ res => not res.isOk) ev)
 
 def memWriteAddrAnnounces (p : PreCand nThreads) : Std.ExtTreeSet Eid :=
-  p.collectEid (fun _ ev => IEvent.is_mem_write_announce ev)
+  p.collectEidWith (fun _ ev => IEvent.is_mem_write_announce ev)
 def memWrites (p : PreCand nThreads) : Std.ExtTreeSet Eid :=
-  p.collectEid (fun _ ev => IEvent.is_mem_write ev)
+  p.collectEidWith (fun _ ev => IEvent.is_mem_write ev)
 def memWriteReqs (p : PreCand nThreads) : Std.ExtTreeSet Eid :=
-  p.collectEid (fun _ ev => IEvent.is_mem_write_req ev)
+  p.collectEidWith (fun _ ev => IEvent.is_mem_write_req ev)
 def memWriteAborts (p : PreCand nThreads) : Std.ExtTreeSet Eid :=
-  p.collectEid (fun _ ev => IEvent.is_mem_write_req_with ev (fun _ _ _ res => not res.isOk))
+  p.collectEidWith (fun _ ev => IEvent.is_mem_write_req_with (fun _ _ _ res => not res.isOk) ev)
+
+def memEvents (p : PreCand nThreads) : Std.ExtTreeSet Eid :=
+  p.memReads ∪ p.memWrites
 
 def readsByKind (p : PreCand nThreads) (q : Arch.mem_acc → Bool)
     : Std.ExtTreeSet Eid :=
-  p.collectEid (fun _ ev => IEvent.is_mem_read_with ev (fun req _ _ => q req.accessKind))
+  p.collectEidWith (fun _ ev => IEvent.is_mem_read_with (fun req _ _ => q req.accessKind) ev)
 def writesByKind (p : PreCand nThreads) (q : Arch.mem_acc → Bool)
     : Std.ExtTreeSet Eid :=
-  p.collectEid (fun _ ev => IEvent.is_mem_write_with ev (fun req _ _ => q req.accessKind))
+  p.collectEidWith (fun _ ev => IEvent.is_mem_write_with (fun req _ _ => q req.accessKind) ev)
 
 def barriers (p : PreCand nThreads) : Std.ExtTreeSet Eid :=
-  p.collectEid (fun _ ev => IEvent.is_barrier ev)
+  p.collectEidWith (fun _ ev => IEvent.is_barrier ev)
 def cacheOps (p : PreCand nThreads) : Std.ExtTreeSet Eid :=
-  p.collectEid (fun _ ev => IEvent.is_cache_op ev)
+  p.collectEidWith (fun _ ev => IEvent.is_cache_op ev)
 def tlbOps (p : PreCand nThreads) : Std.ExtTreeSet Eid :=
-  p.collectEid (fun _ ev => IEvent.is_tlb_op ev)
+  p.collectEidWith (fun _ ev => IEvent.is_tlb_op ev)
 
 def finalThreadRegisterMap (p : PreCand nThreads) (tid : Fin nThreads) : RegisterMap :=
   p.events[tid].foldl (fun regMap iTrace =>
@@ -428,13 +683,6 @@ def finalThreadRegisterMap (p : PreCand nThreads) (tid : Fin nThreads) : Registe
 
 def finalRegisterMaps (p : PreCand nThreads) : Vector RegisterMap nThreads :=
   Vector.ofFn (finalThreadRegisterMap p)
-
--- TODO:
--- gatherByKey (create map of keys to events)
--- sameKey (create equivalence relation)
--- sameThread (equivalence relation)
--- sameInstructionInstance (equiv rel)
--- ...
 
 def collectEidByKey {K : Type} [Ord K] [Std.TransCmp (compare : K → K → Ordering)]
     (p : PreCand nThreads) (getKey : Eid → IEvent → Option K)
@@ -477,10 +725,16 @@ def interInstructionOrder (p : PreCand nThreads) : Rel Eid :=
   |>.filter (fun (a,b) => a.iid < b.iid)
 
 def programOrder (p : PreCand nThreads) : Rel Eid :=
-  Rel.union p.interInstructionOrder p.intraInstructionOrder
+  p.interInstructionOrder ∪ p.intraInstructionOrder
 
 def sameAddr (p : PreCand nThreads) : Rel Eid :=
   p.sameKey (fun _ ev => ev.getAddr)
+
+def sameSize (p : PreCand nThreads) : Rel Eid :=
+  p.sameKey (fun _ ev => ev.getSize)
+
+def sameFootprint (p : PreCand nThreads) : Rel Eid :=
+  p.sameAddr ∩ p.sameSize
 
 def sameMemValue (p : PreCand nThreads) : Rel Eid :=
   p.sameKey (fun _ ev => ev.getMemValue)
@@ -491,9 +745,40 @@ def sameReg (p : PreCand nThreads) : Rel Eid :=
 def sameRegSameValue (p : PreCand nThreads) : Rel Eid :=
   p.sameKey (fun eid ev => Option.map (eid.tid, ·) ev.getRegValue)
 
--- TODO: finish adding other relations starting from is_valid_init_reg_read and co.
+
+def is_valid_init_reg_read (p : PreCand nThreads) (eid : Eid) : Prop :=
+  match p[eid]? with
+  | .some ev =>
+      if h : eid.tid < nThreads then
+        let tid : Fin nThreads := ⟨eid.tid, h⟩
+        ev.is_reg_read_with (fun reg _acc val =>
+          p.init.regs[tid].get? reg = Option.some val)
+      else
+        False
+  | .none => False
+
+instance : Decidable (is_valid_init_reg_read p eid) := by
+  unfold is_valid_init_reg_read
+  split <;> infer_instance
+
+def possibleInitRegReads (p : PreCand nThreads) : Std.ExtTreeSet Eid :=
+  p.collectEidWith (fun eid _ev => p.is_valid_init_reg_read eid)
+
+def is_valid_init_mem_read (p : PreCand nThreads) (eid : Eid) : Prop :=
+  match p[eid]? with
+  | .some ev => ev.is_mem_read_with (fun req val _tags =>
+      p.init.memory.read req.size req.address = val
+    )
+  | .none => False
+
+instance : Decidable (is_valid_init_mem_read p eid) := by
+  unfold is_valid_init_mem_read
+  split <;> infer_instance
+
+-- TODO: `not_after` relation. in this iff `(· ∩ po⁻¹ = ∅)`
 
 end PreCand
+
 
 structure Cand (nThreads : Nat) [Arch] [ArchExtra] where
   pre : PreCand nThreads
@@ -501,7 +786,6 @@ structure Cand (nThreads : Nat) [Arch] [ArchExtra] where
   regReadsFrom : Rel Eid
   coherence : Rel Eid
   exclusives : Rel Eid
-
 
 namespace Cand
 
@@ -545,12 +829,231 @@ def toArchState (c : Cand nThreads) : ArchState nThreads :=
   , regs := c.pre.finalRegisterMaps
   }
 
-def valid_rf (c : Cand nThreads) (wsrc rdst : Eid) : Prop :=
-  Option.isSome (do
-    let write ← c[wsrc]?
-    -- TODO complete this and other similar definitions.
-    return Option.some ()
-  )
+def initMemReads (c : Cand nThreads) : Std.ExtTreeSet Eid :=
+  c.pre.memReads \ c.memReadsFrom.range
+
+def memFromReads (c : Cand nThreads) : Rel Eid :=
+  (Δ c.pre.memReads ; c.pre.sameAddr ; Δ c.pre.memWrites)
+    \ ((c.coherence ∪ Δ c.pre.memWrites) ; c.memReadsFrom)⁻¹
+
+def initRegReads (c : Cand nThreads) : Std.ExtTreeSet Eid :=
+  c.pre.regReads \ c.regReadsFrom.range
+
+def regFromReads (c : Cand nThreads) : Rel Eid :=
+  Δ c.pre.regReads ; c.pre.sameReg ; Δ c.pre.regWrites
+    \ ((c.pre.interInstructionOrder ∪ Δ c.pre.regWrites) ; c.regReadsFrom)⁻¹
+
+def pcReadsFrom (c : Cand nThreads) : Rel Eid :=
+  Δ c.pre.pcWrites ; c.regReadsFrom ; Δ c.pre.pcReads
+
+def regReadsFromData (c : Cand nThreads) : Rel Eid :=
+  c.regReadsFrom \ c.pcReadsFrom
+
+def is_valid_mem_rf_data (c : Cand nThreads) (wsrc rdst : Eid) : Prop :=
+  match (do
+      let write ← c[wsrc]?
+      let wAddr ← write.getAddr
+      let wVal ← write.getMemValue
+      let read ← c[rdst]?
+      let rAddr ← read.getAddr
+      let rVal ← read.getMemValue
+      return (wAddr, wVal, rAddr, rVal)
+    ) with
+  | .some (wAddr, wVal, rAddr, rVal) =>
+    wAddr = rAddr ∧ wVal = rVal
+  | .none => False
+
+instance : Decidable (is_valid_mem_rf_data c wsrc rdst) := by
+  unfold is_valid_mem_rf_data
+  split <;> infer_instance
+
+structure mem_reads_from_wf (c : Cand nThreads) where
+  from_writes : c.memReadsFrom.domain ⊆ c.pre.memWrites
+  to_reads : c.memReadsFrom.range ⊆ c.pre.memReads
+  injective : c.memReadsFrom.injective
+  data_valid : ∀ arrow ∈ c.memReadsFrom, c.is_valid_mem_rf_data arrow.fst arrow.snd
+  initial_data_valid : ∀ eid ∈ c.initMemReads, c.pre.is_valid_init_mem_read eid
+
+theorem mem_reads_from_wf.mk_iff (c : Cand nThreads)
+    : mem_reads_from_wf c
+    ↔ c.memReadsFrom.domain ⊆ c.pre.memWrites
+    ∧ c.memReadsFrom.range ⊆ c.pre.memReads
+    ∧ c.memReadsFrom.injective
+    ∧ (∀ arrow ∈ c.memReadsFrom, c.is_valid_mem_rf_data arrow.fst arrow.snd)
+    ∧ (∀ eid ∈ c.initMemReads, c.pre.is_valid_init_mem_read eid)
+  := by
+  apply Iff.intro
+  · exact fun { from_writes, to_reads, injective, data_valid, initial_data_valid }
+      => ⟨from_writes, to_reads, injective, data_valid, initial_data_valid⟩
+  · exact fun ⟨from_writes, to_reads, injective, data_valid, initial_data_valid⟩
+      => { from_writes, to_reads, injective, data_valid, initial_data_valid }
+
+instance : Decidable (mem_reads_from_wf c) := by
+  rw [mem_reads_from_wf.mk_iff]
+  infer_instance
+
+structure coherence_wf (c : Cand nThreads) where
+  transitive : c.coherence.transitive
+  irreflexive : c.coherence.irreflexive
+  -- TODO: this differs from archsem-rocq. I'm confused in case weid1=weid2 in archsem-rocq.
+  total_over_same_addr :
+    ∀ arrow ∈ c.pre.sameAddr, arrow ∈ c.coherence ∨ arrow.swap ∈ c.coherence
+
+theorem coherence_wf.mk_iff (c : Cand nThreads)
+    : coherence_wf c ↔ c.coherence.transitive ∧ c.coherence.irreflexive ∧ (∀ arrow ∈ c.pre.sameAddr, arrow ∈ c.coherence ∨ arrow.swap ∈ c.coherence)
+  := by
+  apply Iff.intro
+  · exact fun { transitive, irreflexive, total_over_same_addr }
+      => ⟨transitive, irreflexive, total_over_same_addr⟩
+  · exact fun ⟨transitive, irreflexive, total_over_same_addr⟩
+      => { transitive, irreflexive, total_over_same_addr }
+
+instance : Decidable (coherence_wf c) := by
+  rw [coherence_wf.mk_iff]
+  infer_instance
+
+structure exclusives_wf (c : Cand nThreads) where
+  from_reads : c.exclusives.domain ⊆ c.pre.readsByKind Arch.mem_acc_is_exclusive
+  to_writes : c.exclusives.range ⊆ c.pre.writesByKind Arch.mem_acc_is_exclusive
+  instruction_order : c.exclusives ⊆ c.pre.interInstructionOrder
+  same_addr : c.exclusives ⊆ c.pre.sameAddr
+
+/-
+`mk_iff` can be derived automatically with a mathlib attribute but
+we dont depend on mathlib.
+-/
+theorem exclusives_wf.mk_iff (c : Cand nThreads)
+    : exclusives_wf c
+    ↔ c.exclusives.domain ⊆ c.pre.readsByKind Arch.mem_acc_is_exclusive
+    ∧ c.exclusives.range ⊆ c.pre.writesByKind Arch.mem_acc_is_exclusive
+    ∧ c.exclusives ⊆ c.pre.interInstructionOrder
+    ∧ c.exclusives ⊆ c.pre.sameAddr
+  := by
+  apply Iff.intro
+  · exact fun { from_reads, to_writes, instruction_order, same_addr }
+      => ⟨from_reads, to_writes, instruction_order, same_addr⟩
+  · exact fun ⟨from_reads, to_writes, instruction_order, same_addr⟩
+      => { from_reads, to_writes, instruction_order, same_addr }
+
+instance : Decidable (exclusives_wf c) := by
+  rw [exclusives_wf.mk_iff]
+  infer_instance
+
+structure reg_reads_from_wf (c : Cand nThreads) where
+  from_writes : c.regReadsFrom.domain ⊆ c.pre.regWrites
+  to_reads : c.regReadsFrom.range ⊆ c.pre.regReads
+  injective : c.regReadsFrom.injective
+  data_valid : c.regReadsFrom ⊆ c.pre.sameRegSameValue
+  initial_data_valid : c.initRegReads ⊆ c.pre.possibleInitRegReads
+
+theorem reg_reads_from_wf.mk_iff (c : Cand nThreads)
+    : reg_reads_from_wf c
+    ↔ c.regReadsFrom.domain ⊆ c.pre.regWrites
+    ∧ c.regReadsFrom.range ⊆ c.pre.regReads
+    ∧ c.regReadsFrom.injective
+    ∧ c.regReadsFrom ⊆ c.pre.sameRegSameValue
+    ∧ c.initRegReads ⊆ c.pre.possibleInitRegReads
+  := by
+  apply Iff.intro
+  · exact fun { from_writes, to_reads, injective, data_valid, initial_data_valid }
+      => ⟨from_writes, to_reads, injective, data_valid, initial_data_valid⟩
+  · exact fun ⟨from_writes, to_reads, injective, data_valid, initial_data_valid⟩
+      => { from_writes, to_reads, injective, data_valid, initial_data_valid }
+
+instance : Decidable (reg_reads_from_wf c) := by
+  rw [reg_reads_from_wf.mk_iff]
+  infer_instance
+
+def addr_space_wf (c : Cand nThreads) : Prop :=
+  ∀ pair ∈ c.pre.iEventList',
+    match pair.snd.getMemRequest with
+    | .some req => req.addressSpace = c.pre.init.addressSpace
+    | .none => True
+
+instance : Decidable (addr_space_wf c) := by
+  unfold addr_space_wf
+  if h : c.pre.iEventList'.all (fun pair =>
+      match pair.snd.getMemRequest with
+      | .some req => decide (req.addressSpace = c.pre.init.addressSpace)
+      | .none => true) = true then
+    apply Decidable.isTrue
+    intro pair h_pair
+    have h_pair_valid := List.all_eq_true.mp h pair h_pair
+    split at h_pair_valid
+    · exact of_decide_eq_true h_pair_valid
+    · exact True.intro
+  else
+    apply Decidable.isFalse
+    intro h_wf
+    apply h
+    apply List.all_eq_true.mpr
+    intro pair h_pair
+    specialize h_wf pair h_pair
+    cases h_req : pair.snd.getMemRequest with
+    | some req =>
+      simp [h_req] at h_wf ⊢
+      exact h_wf
+    | none =>
+      rfl
+
+-- TODO: `footprint_wf`. I dont understand why archsem rocq strictly needs this.
+
+structure wf (c : Cand nThreads) where
+  only_supported_events : ∀ pair ∈ c.pre.iEventList', ¬ pair.snd.is_unsupported_event
+  addr_space : addr_space_wf c
+  mem_reads_from : mem_reads_from_wf c
+  coherence : coherence_wf c
+  exclusives : exclusives_wf c
+  reg_reads_from : reg_reads_from_wf c
+
+theorem wf.mk_iff (c : Cand nThreads)
+    : wf c
+    ↔ (∀ pair ∈ c.pre.iEventList', ¬ pair.snd.is_unsupported_event)
+    ∧ addr_space_wf c
+    ∧ mem_reads_from_wf c
+    ∧ coherence_wf c
+    ∧ exclusives_wf c
+    ∧ reg_reads_from_wf c
+  := by
+  apply Iff.intro
+  · exact fun { only_supported_events, addr_space, mem_reads_from, coherence, exclusives, reg_reads_from }
+      => ⟨only_supported_events, addr_space, mem_reads_from, coherence, exclusives, reg_reads_from⟩
+  · exact fun ⟨only_supported_events, addr_space, mem_reads_from, coherence, exclusives, reg_reads_from⟩
+      => { only_supported_events, addr_space, mem_reads_from, coherence, exclusives, reg_reads_from }
+
+instance : Decidable (wf c) := by
+  rw [wf.mk_iff]
+  infer_instance
+
+-- TODO: CR clang for thibaut: symbol presicence for rocq?
+def intra_instruction_order_addr (c : Cand nThreads) : Rel Eid :=
+  c.pre.intraInstructionOrder ;
+  ((Δ c.pre.memWriteAddrAnnounces ; c.pre.intraInstructionOrder ; Δ c.pre.memWriteReqs
+   ∩ c.pre.sameFootprint) ∪ Δ c.pre.memReads)
+
+def addr (c : Cand nThreads) : Rel Eid :=
+  Δ c.pre.memReads ;
+  (Δ c.pre.memReads ∪ (c.pre.intraInstructionOrder ; c.regReadsFromData)⁺) ;
+  c.pre.intraInstructionOrder ;
+  Δ c.pre.memEvents
+
+
+def data (c : Cand nThreads) : Rel Eid :=
+  Δ c.pre.memReads ;
+  (Δ c.pre.memReads ∪ (c.pre.intraInstructionOrder ; c.regReadsFromData)⁺) ;
+  c.pre.intraInstructionOrder ;
+  Δ c.pre.memWriteReqs
+
+def ctrl (c : Cand nThreads) : Rel Eid :=
+  Δ c.pre.memReads ;
+  (Δ c.pre.memReads ∪ (c.pre.intraInstructionOrder ; c.regReadsFromData)⁺) ;
+  c.pre.intraInstructionOrder ;
+  Δ c.pre.memWriteReqs
+
+def atomicUpdate (c : Cand nThreads) : Rel Eid :=
+  c.pre.sameInstructionInstance ∩
+  (PreCand.setProd (c.pre.memReads) (c.pre.memWrites)) ∩
+  c.pre.sameFootprint
 
 end Cand
 
@@ -558,6 +1061,7 @@ inductive AxiomaticModel.Behavior (Flag : Type) where
   | allowed
   | rejected
   | flagged (f : Flag)
+deriving Repr
 
 def AxiomaticModel [Arch] [ArchExtra] (Flag : Type)
   := (nThreads : Nat) → Cand nThreads
