ArchSemTinyArm/SequentialAxiomatic.lean
@@ -1,0 +1,108 @@
+-- SPDX-FileCopyrightText: 2026 Christopher Lang
+--
+-- SPDX-License-Identifier: Apache-2.0 OR BSD-2-Clause
+
+import ArchSem.Defs
+import ArchSem.CandidateExecution
+import ArchSemTinyArm.Defs
+
+open ArchSem.CandidateExecutions
+open ArchSem.TerminatingModel
+
+namespace ArchSemTinyArm.SequentialAxiomatic
+
+section DerivedRelations
+
+variable (c : Cand nThreads)
+
+abbrev int := c.pre.sameThread
+abbrev iio := c.pre.intraInstructionOrder
+
+abbrev RR := c.pre.regReads
+abbrev RW := c.pre.regWrites
+abbrev RE := RR c ∪ RW c
+abbrev rrf := c.regReadsFrom
+abbrev rfr := c.regFromReads
+
+abbrev W := c.pre.memWrites
+abbrev R := c.pre.memReads
+abbrev M := (c.pre.readsByKind mem_acc_is_explicit) ∪ (c.pre.writesByKind mem_acc_is_explicit)
+abbrev T := c.pre.readsByKind mem_acc_is_ttw
+abbrev IF := c.pre.readsByKind mem_acc_is_ifetch
+abbrev IR := c.initMemReads
+
+def amo := c.atomicUpdate
+def rmw := c.exclusives ∪ amo c
+
+-- If we were mixed size we would need to re-think coherence.
+def co := Δ W c ; c.coherence ; Δ W c ∩ c.pre.sameAddr
+def coi := co c ∩ int c
+def coe := co c \ coi c
+
+def rf := c.memReadsFrom ; Δ R c
+def rfi := rf c ∩ int c
+def rfe := rf c \ rfi c
+def fr := Δ R c ; c.memFromReads
+def fri := fr c ∩ int c
+def fre := fr c \ fri c
+
+def po := c.pre.programOrder
+
+def TE := c.pre.collectEidWith (fun _ ev => ev.is_arch_exception)
+def ERET := c.pre.collectEidWith (fun _ ev => ev.is_return_exception)
+
+end DerivedRelations
+
+structure consistent (c : Cand nThreads) where
+  total : Rel.acyclic (po c ∪ fr c ∪ co c ∪ rf c ∪ rfr c ∪ rrf c)
+  atomic : ∅ = (rmw c ∩ (fre c ; coe c))
+
+-- TODO: ArchSem rocq has a register whitelist. I dont understand why.
+structure not_ub (c : Cand nThreads) where
+  initial_reads : (T c ∪ IF c) ⊆ IR c
+  register_write_permitted : ∅ = c.pre.collectEidWith (fun _ ev => ev.is_reg_write_with (fun _ acc _ => acc.isSome))
+  register_read_permitted : ∅ = c.pre.collectEidWith (fun _ ev => ev.is_reg_read_with (fun _ acc _ => acc.isSome))
+  memory_events_permitted : c.pre.memEvents ⊆ M c ∪ T c ∪ IF c
+  no_exceptions : ∅ = TE c ∪ ERET c
+
+theorem consistent.mk_iff (c : Cand nThreads)
+    : consistent c
+    ↔ Rel.acyclic (po c ∪ fr c ∪ co c ∪ rf c ∪ rfr c ∪ rrf c)
+    ∧ ∅ = (rmw c ∩ (fre c ; coe c))
+  := by
+  apply Iff.intro
+  · exact fun { total, atomic } => ⟨total, atomic⟩
+  · exact fun ⟨total, atomic⟩ => { total, atomic }
+
+theorem not_ub.mk_iff (c : Cand nThreads)
+    : not_ub c
+    ↔ (T c ∪ IF c) ⊆ IR c
+    ∧ ∅ = c.pre.collectEidWith (fun _ ev => ev.is_reg_write_with (fun _ acc _ => acc.isSome))
+    ∧ ∅ = c.pre.collectEidWith (fun _ ev => ev.is_reg_read_with (fun _ acc _ => acc.isSome))
+    ∧ c.pre.memEvents ⊆ M c ∪ T c ∪ IF c
+    ∧ ∅ = TE c ∪ ERET c
+  := by
+  apply Iff.intro
+  · exact fun { initial_reads, register_write_permitted, register_read_permitted, memory_events_permitted, no_exceptions }
+      => ⟨initial_reads, register_write_permitted, register_read_permitted, memory_events_permitted, no_exceptions⟩
+  · exact fun ⟨ initial_reads, register_write_permitted, register_read_permitted, memory_events_permitted, no_exceptions ⟩
+      => { initial_reads, register_write_permitted, register_read_permitted, memory_events_permitted, no_exceptions }
+
+instance : Decidable (consistent c) := by
+  rw [consistent.mk_iff]
+  infer_instance
+
+instance : Decidable (not_ub c) := by
+  rw [not_ub.mk_iff]
+  infer_instance
+
+def model : AxiomaticModel Empty := fun _ c =>
+  if consistent c then
+    if not_ub c then
+      .ok .allowed
+    else
+      .error "undefined behaviour"
+  else
+    .ok .rejected
+
+end ArchSemTinyArm.SequentialAxiomatic
